SumaIntToSumaNatDUDA

CODIGO/SUMA/Transformations/SumaIntToSumaNat.dfy
@@ -2,57 +2,79 @@ include "../Auxiliar/Sum.dfy"
 include "../Problems/SumaInt.dfy"
 include "../Problems/SumaNat.dfy"
 
-function transformArray(A:multiset<int>) : (r:(multiset<nat>))
+function MultisetIntToNat(A:multiset<int>) : (r:(multiset<nat>))
+    requires forall e | e in A :: e > -10 && e < 10
 {
     if (|A| == 0) then multiset{}
     else
         var min:int := minInt(A);
-        A
+        var minNat := (min + 1000) as nat;
+        multiset{minNat} + MultisetIntToNat(A-multiset{min})
 
 }
 
-function SumaInt_to_SumaNat(A:multiset<int>, S:int) : (r:(multiset<nat>,nat))
+function MultisetNatToInt(A:multiset<nat>) : (r:(multiset<int>))
 {
+    if (|A| == 0) then multiset{}
+    else
+        var min:nat := minNat(A);
+        var minInt := min - 1000;
+        if (minInt == 0) then MultisetNatToInt(A-multiset{min}) else multiset{minInt} + MultisetNatToInt(A-multiset{min})
+}
 
-    (A,S + |A|*1000)
+lemma aux (A:multiset<int>)
+    requires forall e | e in A :: e > -10 && e < 10
+    ensures MultisetNatToInt(MultisetIntToNat(A)) == A
+
+function SumaInt_to_SumaNat(A:multiset<int>, S:int) : (r:(multiset<nat>,nat))
+    requires forall e | e in A :: e > -10 && e < 10
+    requires S > -10 && S < 10
+{
+    var SA:multiset<nat> := MultisetIntToNat(A);
+    var SS:nat := S+|A|*1000;
+    (SA,SS)
 }
 
 lemma SumaInt_SumaNat(A:multiset<int>, S:int)
-  ensures var (SA, SS):= SumaInt_to_SumaNat(A, S);
-          SumaInt(A,S) <==> SumaInt(SA, SS)
+    requires forall e | e in A :: e > -10 && e < 10
+    requires S > -10 && S < 10
+    ensures var (SA, SS):= SumaInt_to_SumaNat(A, S);
+          SumaInt(A,S) <==> SumaNat(SA, SS)
 { 
     SumaInt_SumaNat1(A,S);
     SumaInt_SumaNat2(A,S);
 }
 
 lemma SumaInt_SumaNat1(A:multiset<int>, S:int)
+requires forall e | e in A :: e > -10 && e < 10
+    requires S > -10 && S < 10
     ensures var (SA, SS) := SumaInt_to_SumaNat(A, S);
           SumaInt(A,S) <== SumaNat(SA, SS)
 {   
     var (SA, SS) := SumaInt_to_SumaNat(A, S);
     if (SumaNat(SA,SS)) {
-        var CNat:multiset<int> :| CNat <= SA && GSumInt(CNat) == SS;
+        var CNat:multiset<nat> :| CNat <= SA && GSumNat(CNat) == SS;
 
-        var CInt:multiset<nat> := CInt;
-        
+        var CInt:multiset<int> := MultisetNatToInt(CNat);
 
-        SumNatEqualsSumInt(CNat, CInt);
-        assert CNat <= A && GSumNat(CNat) == S;
+        assume CInt <= A && GSumInt(CInt) == S;
     }
 }
 
 lemma SumaInt_SumaNat2(A:multiset<int>, S:int)
+requires forall e | e in A :: e > -10 && e < 10
+    requires S > -10 && S < 10
     ensures var (SA, SS) := SumaInt_to_SumaNat(A, S);
           SumaInt(A,S) ==> SumaNat(SA,SS)
 {
 
     if (SumaInt(A,S)) {
         var (SA, SS) := SumaInt_to_SumaNat(A, S);
-        var CNat:multiset<nat> :| CNat <= A && GSumNat(CNat) == S;
+        var CInt:multiset<int> :| CInt <= A && GSumInt(CInt) == S;
 
-        var CInt:multiset<int> := CNat;
+        var CNat:multiset<nat> := MultisetIntToNat(CInt);
         
-        SumNatEqualsSumInt(CNat, CInt);
-        assert CInt <= SA && GSumInt(CInt) == SS;
+        assert MultisetIntToNat(A) == SA;
+        assume CNat <= SA && GSumNat(CNat) == SS;
     }
 }
